PAC_Checker_LLVM/Assn_Env.thy
@@ -1,0 +1,201 @@
+theory Assn_Env
+  imports Isabelle_LLVM.IICF
+begin
+
+text \<open>This theory defines a hierarchy of locales on refinement assertions
+  to avoid code duplication.\<close>
+
+section \<open>Generic bridge from \<open>hfref\<close> rules to Hoare triples\<close>
+
+text \<open>The locale assumptions below are refinement rules (\<open>hfref\<close>). 
+  \<open>vgc\<close>, however, works with Hoare triples. Therefore we might want
+  a translation of _hnr rules to vcg_rules\<close>
+
+lemma hfref_htriple_k1:
+  assumes R: \<open>(f, RETURN o g) \<in> A\<^sup>k \<rightarrow>\<^sub>a B\<close>
+  shows \<open>llvm_htriple (A a ai) (f ai) (\<lambda>r. A a ai ** B (g a) r)\<close>
+proof -
+  note HNR = R[to_hnr, unfolded autoref_tag_defs]
+  note HT = HNR[THEN hn_refineD]
+  show ?thesis
+    apply (rule htriple_ent_pre[OF _ htriple_ent_post[OF _ HT]])
+    unfolding hn_ctxt_def
+    apply (rule entails_refl)
+    subgoal by (auto simp: entails_def sep_algebra_simps pred_lift_extract_simps
+      sep_conj_exists pw_le_iff refine_pw_simps)
+    subgoal by simp
+    done
+qed
+
+lemma hfref_htriple_k2:
+  assumes R: \<open>(uncurry f, uncurry (RETURN oo g)) \<in> A\<^sup>k *\<^sub>a B\<^sup>k \<rightarrow>\<^sub>a C\<close>
+  shows \<open>llvm_htriple (A a ai ** B b bi) (f ai bi) (\<lambda>r. A a ai ** B b bi ** C (g a b) r)\<close>
+proof -
+  note HNR = R[to_hnr, unfolded autoref_tag_defs]
+  note HT = HNR[THEN hn_refineD]
+  show ?thesis
+    apply (rule htriple_ent_pre[OF _ htriple_ent_post[OF _ HT]])
+    unfolding hn_ctxt_def
+    apply (rule entails_refl)
+    subgoal by (auto simp: entails_def sep_algebra_simps pred_lift_extract_simps
+      sep_conj_exists pw_le_iff refine_pw_simps)
+    subgoal by simp
+    done
+qed
+
+section \<open>Copying\<close>
+
+(* Copying setup is taken from the sorting examples in Isabelle-LLVM *)
+
+definition \<open>is_copy A cp \<equiv> (cp, RETURN o COPY) \<in> A\<^sup>k \<rightarrow>\<^sub>a A\<close>
+
+lemma is_copy_hnr[sepref_fr_rules]:
+  \<open>GEN_ALGO cp (is_copy A) \<Longrightarrow> (cp, RETURN o COPY) \<in> A\<^sup>k \<rightarrow>\<^sub>a A\<close>
+  unfolding is_copy_def GEN_ALGO_def by auto
+
+lemma is_copy_pure_gen_algo: \<open>CONSTRAINT is_pure A \<Longrightarrow> GEN_ALGO Mreturn (is_copy A)\<close>
+  unfolding is_copy_def GEN_ALGO_def
+  by (rule hnr_pure_COPY)
+
+section \<open>The locale hierarchy\<close>
+
+subsection \<open>Freeable assertions\<close>
+
+locale freeable_assn =
+  fixes A :: \<open>'a \<Rightarrow> 'b::llvm_rep \<Rightarrow> assn\<close>
+    and afree :: \<open>'b \<Rightarrow> unit llM\<close>
+  assumes afree_free[sepref_frame_free_rules]: \<open>MK_FREE A afree\<close>
+begin
+
+lemma afree_rule[vcg_rules]: \<open>llvm_htriple (A a c) (afree c) (\<lambda>_. \<box>)\<close>
+  by (rule MK_FREED[OF afree_free])
+
+end
+
+subsection \<open>Copyable assertions\<close>
+
+locale copyable_assn = freeable_assn +
+  fixes acopy :: \<open>'b::llvm_rep \<Rightarrow> 'b llM\<close>
+  assumes acopy_hnr[sepref_fr_rules]: \<open>(acopy, RETURN o COPY) \<in> A\<^sup>k \<rightarrow>\<^sub>a A\<close>
+begin
+
+lemma acopy_is_copy: \<open>is_copy A acopy\<close>
+  unfolding is_copy_def by (rule acopy_hnr)
+
+lemma acopy_gen_algo[sepref_gen_algo_rules]: \<open>GEN_ALGO acopy (is_copy A)\<close>
+  unfolding GEN_ALGO_def by (rule acopy_is_copy)
+
+lemma acopy_rule[vcg_rules]: \<open>llvm_htriple (A a c) (acopy c) (\<lambda>r. A a c ** A a r)\<close>
+  using hfref_htriple_k1[OF acopy_hnr] by simp
+
+end
+
+subsection \<open>Assertions with an equality test\<close>
+
+locale eq_assn =
+  fixes A :: \<open>'a \<Rightarrow> 'b::llvm_rep \<Rightarrow> assn\<close>
+    and aeq :: \<open>'b \<Rightarrow> 'b \<Rightarrow> 1 word llM\<close>
+  assumes aeq_hnr[sepref_fr_rules]:
+      \<open>(uncurry aeq, uncurry (RETURN oo (=))) \<in> A\<^sup>k *\<^sub>a A\<^sup>k \<rightarrow>\<^sub>a bool1_assn\<close>
+begin
+
+lemma aeq_rule[vcg_rules]:
+  \<open>llvm_htriple (A a ai ** A b bi) (aeq ai bi) (\<lambda>r. A a ai ** A b bi ** bool1_assn (a = b) r)\<close>
+  by (rule hfref_htriple_k2[OF aeq_hnr])
+
+end
+
+subsection \<open>Linearly ordered assertions\<close>
+
+locale linorder_assn = eq_assn A aeq
+  for A :: \<open>'a::linorder \<Rightarrow> 'b::llvm_rep \<Rightarrow> assn\<close>
+  and aeq :: \<open>'b \<Rightarrow> 'b \<Rightarrow> 1 word llM\<close> +
+  fixes alt :: \<open>'b \<Rightarrow> 'b \<Rightarrow> 1 word llM\<close>
+  assumes alt_hnr[sepref_fr_rules]:
+      \<open>(uncurry alt, uncurry (RETURN oo (<))) \<in> A\<^sup>k *\<^sub>a A\<^sup>k \<rightarrow>\<^sub>a bool1_assn\<close>
+begin
+
+lemma alt_rule[vcg_rules]:
+  \<open>llvm_htriple (A a ai ** A b bi) (alt ai bi) (\<lambda>r. A a ai ** A b bi ** bool1_assn (a < b) r)\<close>
+  by (rule hfref_htriple_k2[OF alt_hnr])
+
+end
+
+subsection \<open>Combination: copyable and linearly ordered\<close>
+
+locale linorder_copyable_assn =
+  copyable_assn A afree acopy + linorder_assn A aeq alt
+  for A :: \<open>'a::linorder \<Rightarrow> 'b::llvm_rep \<Rightarrow> assn\<close>
+  and afree :: \<open>'b \<Rightarrow> unit llM\<close>
+  and acopy :: \<open>'b \<Rightarrow> 'b llM\<close>
+  and aeq alt :: \<open>'b \<Rightarrow> 'b \<Rightarrow> 1 word llM\<close>
+
+subsection \<open>Hashable assertions\<close>
+
+locale hashable_assn =
+  fixes A :: \<open>'a \<Rightarrow> 'b::llvm_rep \<Rightarrow> assn\<close>
+    and ahash :: \<open>'a \<Rightarrow> 64 word\<close>
+    and ahash_impl :: \<open>'b \<Rightarrow> 64 word llM\<close>
+  assumes Ahash_hnr[sepref_fr_rules]:
+    \<open>(ahash_impl, RETURN o ahash) \<in> A\<^sup>k \<rightarrow>\<^sub>a word_assn' TYPE(64)\<close>
+begin
+
+lemma Ahash_rule[vcg_rules]:
+  \<open>llvm_htriple (A a ai) (ahash_impl ai) (\<lambda>r. A a ai ** word_assn' TYPE(64) (ahash a) r)\<close>
+  by (rule hfref_htriple_k1[OF Ahash_hnr])
+
+end
+
+section \<open>Regression tests\<close>
+
+text \<open>Instantiate the hierarchy with 64-bit \<open>snat\<close> numbers (a pure assertion, so
+  free is a no-op and copy is \<open>Mreturn\<close>) to validate that the assumptions are
+  dischargeable and that the diamond in \<open>linorder_copyable_assn\<close> merges.\<close>
+
+experiment
+begin
+
+interpretation P: copyable_assn \<open>snat_assn' TYPE(64)\<close> \<open>\<lambda>_. Mreturn ()\<close> Mreturn
+  apply unfold_locales
+  subgoal by (rule mk_free_pure)
+  subgoal by (rule hnr_pure_COPY) simp
+  done
+
+interpretation N: linorder_assn \<open>snat_assn' TYPE(64)\<close> ll_icmp_eq ll_icmp_slt
+  apply unfold_locales
+  subgoal by (rule hn_snat_ops(7))
+  subgoal by (rule hn_snat_ops(10))
+  done
+
+end
+
+text \<open>The combined locale, interpreted in a fresh context (with \<open>copyable_assn\<close> or
+  \<open>linorder_assn\<close> already interpreted at the same parameters, \<open>interpretation\<close> only
+  generates obligations for the parts that are new).\<close>
+
+experiment
+begin
+
+interpretation NP: linorder_copyable_assn
+  \<open>snat_assn' TYPE(64)\<close> \<open>\<lambda>_. Mreturn ()\<close> Mreturn ll_icmp_eq ll_icmp_slt
+  apply unfold_locales
+  subgoal by (rule mk_free_pure)
+  subgoal by (rule hnr_pure_COPY) simp
+  subgoal by (rule hn_snat_ops(7))
+  subgoal by (rule hn_snat_ops(10))
+  done
+
+end
+
+experiment
+begin
+
+interpretation E: eq_assn \<open>snat_assn' TYPE(64)\<close> ll_icmp_eq
+  by unfold_locales (rule hn_snat_ops(7))
+
+interpretation L: linorder_assn \<open>snat_assn' TYPE(64)\<close> ll_icmp_eq ll_icmp_slt
+  by unfold_locales (rule hn_snat_ops(10))
+
+end
+
+end
